examples/test2.smt2
@@ -1,0 +1,4 @@
+(set-logic UFLIA)
+(assert (not (or true false)))
+(check-sat)
+(exit)
